compiler/backend/semantics/bviSemScript.sml
@@ -32,7 +32,7 @@ val bvl_to_bvi_def = Define `
             ; ffi := s.ffi |>`;
 
 val small_enough_int_def = Define `
-  small_enough_int i <=> -1073741823 <= i /\ i <= 1073741823`;
+  small_enough_int i <=> -268435457 <= i /\ i <= 268435457`;
 
 val do_app_aux_def = Define `
   do_app_aux op (vs:bvlSem$v list) (s:'ffi bviSem$state) =
