compiler/eval/compilerComputeLib.sml
@@ -341,12 +341,13 @@ in
   (* bvp_to_word *)
   ; add_thms
     [bvp_to_wordTheory.adjust_var_def
-    ,bvp_to_wordTheory.compile_def
-    ,bvp_to_wordTheory.compile_part_def
-    ,bvp_to_wordTheory.assign_def
-    ,bvp_to_wordTheory.comp_def
     ,bvp_to_wordTheory.adjust_set_def
     ,bvp_to_wordTheory.Unit_def
+    ,bvp_to_wordTheory.GiveUp_def
+    ,bvp_to_wordTheory.assign_def
+    ,bvp_to_wordTheory.comp_def
+    ,bvp_to_wordTheory.compile_part_def
+    ,bvp_to_wordTheory.compile_def
     ]
   (*wordLang word_to_word*)
   ; add_thms
